Universe handling in a separate folder

rupicola/io/QExp.fsti
@@ -4,134 +4,117 @@ open FStar.Tactics
 open FStar.Universe
 open Free
 
-noeq
-type uType : Type u#2 =
-| U0 : Type u#0 -> uType
-| U1 : Type u#1 -> uType
-
-let (^->) (a b:uType) : uType =
-  match a, b with
-  | U0 a, U0 b -> U0 (a -> b)
-  | U0 a, U1 b -> U1 (a -> b)
-  | U1 a, U0 b -> U1 (a -> b)
-  | U1 a, U1 b -> U1 (a -> b)
-
-let get_Type (a:uType) : Type u#1 =
-  match a with
-  | U0 a -> ((raise_t unit) -> a)
-  | U1 a -> ((raise_t unit) -> a)
-
 (** typ_env is a typing environment: variables to F* types **)
-type typ_env = nat -> option uType
+type typ_env = nat -> option Type0
 val empty : typ_env
-val extend : uType -> typ_env -> typ_env
+val extend : Type0 -> typ_env -> typ_env
 
 (** eval_env is an evaluation environment: variables to F* values **)
 val eval_env (g:typ_env) : Type
-val hd : #t:uType -> #g:_ -> eval_env (extend t g) -> get_Type t
-val tail : #t:uType -> #g:_ ->  eval_env (extend t g) -> eval_env g
+val hd : #t:Type0 -> #g:_ -> eval_env (extend t g) -> t
+val tail : #t:Type0 -> #g:_ ->  eval_env (extend t g) -> eval_env g
 
-type fs_oexp (g:typ_env) (a:uType) =
-  eval_env g -> get_Type a
-
-#push-options "--print_implicits --print_universes"
-
-(**
-val myf : (#g:typ_env) -> #a:uType -> fs_oexp g a -> eval_env g -> (match a with | U0 b -> b | U1 b -> b)
-
-let myf (#g:typ_env) (#a:uType) (s:fs_oexp g a) (fsG:eval_env g) =
-  match a with
-  | U0 b -> (let s' : eval_env g -> b = s in s' fsG)
-  | U1 b -> (let s' : eval_env g -> b = s in s' fsG)
-**)
-
-let fapp (a b:uType) (f:get_Type (a ^-> b)) (x:get_Type a) : get_Type b =
-  match a ^-> b, a, b with
-  | U0 ab, U0 a, U0 b -> begin
-    let f : get_Type (U0 ab) = f in
-    let f : raise_t unit -> a -> b = f in
-    let x : raise_t unit -> _ = x in
-    (fun tt -> (f tt) (x tt))
-  end
-  | U1 ab, U0 a, U1 b
-  | U1 ab, U1 a, U0 b
-  | U1 ab, U1 a, U1 b -> begin
-    let f : get_Type (U1 ab) = f in
-    let f : raise_t unit -> a -> b = f in
-    let x : raise_t unit -> _ = x in
-    (fun tt -> (f tt) (x tt))
-  end
+type fs_oexp (g:typ_env) (a:Type0) =
+  eval_env g -> a
 
 noeq
-type exp_quotation : #a:uType -> g:typ_env -> fs_oexp g a -> Type =
-| Qtt : #g:typ_env -> exp_quotation #(U0 unit) g (fun _ _ -> ())
-| QFalse : #g:typ_env -> exp_quotation #(U0 bool) g (fun _ _ -> false)
+type exp_quotation : #a:Type0 -> g:typ_env -> fs_oexp g a -> Type =
+| Qtt : #g:typ_env -> exp_quotation g (fun _ -> ())
+| QFalse : #g:typ_env -> exp_quotation g (fun _ -> false)
 
-| QTrue : #g:typ_env -> exp_quotation #(U0 bool) g (fun _ _ -> true)
+| QTrue : #g:typ_env -> exp_quotation g (fun _ -> true)
 
 | QIf : #g:typ_env ->
-        #a:uType ->
-        #cond:fs_oexp g (U0 bool) -> #b1:fs_oexp g a -> #b2:fs_oexp g a ->
+        #a:Type0 ->
+        #cond:fs_oexp g bool -> #b1:fs_oexp g a -> #b2:fs_oexp g a ->
         exp_quotation g cond -> exp_quotation g b1 -> exp_quotation g b2 ->
-        exp_quotation #a g (fun fsG -> if cond fsG (raise_val ()) then b1 fsG else b2 fsG)
+        exp_quotation #a g (fun fsG -> if cond fsG then b1 fsG else b2 fsG)
 
-| QVar0  : #g:typ_env -> #a:uType -> exp_quotation (extend a g) (fun fsG -> hd fsG)
+| QVar0  : #g:typ_env -> #a:Type0 -> exp_quotation (extend a g) (fun fsG -> hd fsG)
 
-| QVar1  : #g:typ_env -> #a:uType -> #b:uType -> exp_quotation (extend b (extend a g)) (fun fsG -> hd (tail fsG))
+| QVar1  : #g:typ_env -> #a:Type0 -> #b:Type0 -> exp_quotation (extend b (extend a g)) (fun fsG -> hd (tail fsG))
 
 (** ... we need a case for each deBrujin variable **)
-| QApp : #g:_ -> #a:uType -> #b:uType ->
-        #f:fs_oexp g (a ^-> b) -> #x:fs_oexp g a ->
+| QApp : #g:_ -> #a:Type0 -> #b:Type0 ->
+        #f:fs_oexp g (a -> b) -> #x:fs_oexp g a ->
         exp_quotation g f -> exp_quotation g x ->
-        exp_quotation #b g (fun fsG -> fapp a b (f fsG) (x fsG))
+        exp_quotation #b g (fun fsG -> (f fsG) (x fsG))
 
-| QLambda : #g:_ -> #a:uType -> #b:uType ->
-        #f:fs_oexp g (a ^-> b) ->
-        exp_quotation #b (extend a g) (fun fsG -> fapp a b (f (tail fsG)) (hd fsG)) ->
+| QLambda : #g:_ -> #a:Type0 -> #b:Type0 ->
+        #f:fs_oexp g (a -> b) ->
+        exp_quotation #b (extend a g) (fun fsG -> (f (tail fsG)) (hd fsG)) ->
         exp_quotation g f
 
 | QFreeReturn :
         #g:typ_env ->
         #a:Type0 ->
-        exp_quotation #(U1 (a -> free a)) g (fun _ _ -> free_return #a)
+        exp_quotation #(a -> free a) g (fun _ -> free_return #a)
 
 | QFreeBind :
         #g:typ_env ->
         #a:Type0 ->
         #b:Type0 ->
-        exp_quotation #(U1 (free a -> (a -> free b) -> free b)) g (fun _ _ -> free_bind #a #b)
+        exp_quotation #(free a -> (a -> free b) -> free b) g (fun _ -> free_bind #a #b)
 
 | QFreeRead :
         #g:typ_env ->
-        exp_quotation #(U1 (unit -> free bool)) g (fun _ _ -> free_read)
+        exp_quotation #(unit -> free bool) g (fun _ -> free_read)
 
 | QFreeWrite :
         #g:typ_env ->
-        exp_quotation #(U1 (bool -> free unit)) g (fun _ _ -> free_write)
+        exp_quotation #(bool -> free unit) g (fun _ -> free_write)
 
 open ExamplesIO
 
-type closed_exp_quotation0 (a:Type u#0) (x:a) =
-  exp_quotation #(U0 a) empty (fun _ _ -> x)
-
-type closed_exp_quotation1 (a:Type u#1) (x:a) =
-  exp_quotation #(U1 a) empty (fun _ _ -> x)
+type closed_exp_quotation (a:Type0) (x:a) =
+  exp_quotation #a empty (fun _ -> x)
 
 #push-options "--no_smt"
 
-let test_u_return ()
-  : Tot (closed_exp_quotation1 _ u_return)
-  by (norm [delta_only [`%u_return; `%fapp; `%op_Hat_Subtraction_Greater]; iota])
+let test_u_return
+  : closed_exp_quotation _ u_return
   = QApp QFreeReturn QTrue
 
-let test_papply_free_return ()
-  : Tot (closed_exp_quotation1 _ papply_free_return)
-  by (norm [delta_only [`%papply_free_return; `%fapp; `%op_Hat_Subtraction_Greater]])
+let test_papply_free_return
+  : closed_exp_quotation _ papply_free_return
   = QFreeReturn
 
-// TODO: why doesn't this work?
-let test_apply_free_return ()
-  : Tot (closed_exp_quotation1 _ apply_free_return)
-  by (norm [delta_only [`%apply_free_return; `%fapp; `%op_Hat_Subtraction_Greater]];
-    dump "H")
-  = QLambda #_ #(U0 bool) #(U1 (free bool)) (QApp QFreeReturn QVar0)
+let test_apply_free_return
+  : closed_exp_quotation _ apply_free_return
+  = QLambda (QApp QFreeReturn QVar0)
+
+let test_apply_free_read
+  : closed_exp_quotation _ apply_free_read
+  = QApp QFreeRead Qtt
+
+let test_apply_free_write_const
+  : closed_exp_quotation _ apply_free_write_const
+  = QApp QFreeWrite QTrue
+
+let test_apply_free_write
+  : closed_exp_quotation _ apply_free_write
+  = QLambda (QApp QFreeWrite QVar0)
+
+let test_apply_free_bind_pure_if ()
+  : closed_exp_quotation _ apply_free_bind_pure_if
+  = magic ()
+//    QLambda
+//       (QApp
+//         (QApp 
+//           QFreeBind
+//           (QApp QFreeReturn QVar0))
+//         (QLambda
+//           (QIf QVar0
+//             (QApp QFreeReturn QFalse)
+//             (QApp QFreeReturn QTrue))))
+
+let test_apply_free_bind_write
+  : closed_exp_quotation _ apply_free_bind_write
+  = magic ()
+//   = QLambda (
+//       QApp 
+//         (QApp 
+//           QFreeBind
+//           (QApp QFreeReturn QVar0))
+//         (QLambda
+//           (QApp QFreeWrite QVar0)))
